omni semantics lemmas

src/Sound/Semantics/Omni.dfy
@@ -1,13 +1,9 @@
 module Omni {
   import opened Defs
   export
-    provides Defs
+    provides Defs, SeqLemma, SeqChoiceLemma
     reveals Sem, SeqSem, VarDeclWitness
 
-  // least predicate VarDeclWitness(s: Stmt, a: State, v: Variable, post: iset<State>, post': iset<State>) {
-  //   && (forall out <- post' :: out - {v} in post)
-  //   && (forall b: Value :: Sem(s, a.Update(v, b), post'))
-  // }
 
   least predicate VarDeclWitness(st: State, v: Variable, post: iset<State>) {
     st - {v} in post
@@ -23,9 +19,96 @@ module Omni {
     case Choice(s0, s1) => Sem(s0, st, post) && Sem(s1, st, post)
   }
 
+  ghost function WP(s: Stmt, post: iset<State>) : iset<State> {
+    iset st: State | Sem(s, st, post)
+  }
+
   least predicate SeqSem(ss: seq<Stmt>, st: State, post: iset<State>) {
     if ss == [] then st in post else
     forall post': iset<State> :: 
       (forall st: State :: SeqSem(ss[1..], st, post) ==> st in post') ==> Sem(ss[0], st, post')
   }
+
+  ghost function SeqWP(ss: seq<Stmt>, post: iset<State>): iset<State> {
+    iset st: State | SeqSem(ss, st, post)
+  }
+
+  lemma SemCons(s: Stmt, st: State, post: iset<State>, post': iset<State>)
+    requires Sem(s, st, post)
+    requires post <= post'
+    ensures Sem(s, st, post')
+  {
+    match s
+    case VarDecl(v, s) =>
+      assert (iset st': State | VarDeclWitness(st', v, post)) <= (iset st': State | VarDeclWitness(st', v, post'));
+    case Seq(ss) => SeqSemCons(ss, st, post, post');
+    case _ =>
+  }
+
+  lemma SeqSemCons(ss: seq<Stmt>, st: State, post: iset<State>, post': iset<State>)
+    requires SeqSem(ss, st, post)
+    requires post <= post'
+    ensures SeqSem(ss, st, post')
+  {
+
+  }
+
+  lemma SemNest(s: Stmt, ss: seq<Stmt>, st: State, post: iset<State>) 
+    requires SeqSem([s] + ss, st, post)
+    ensures Sem(s, st, SeqWP(ss, post))
+  {
+    assert ([s] + ss)[0] == s;
+  }
+
+  lemma SemUnNest(s: Stmt, ss: seq<Stmt>, st: State, post: iset<State>) 
+    requires Sem(s, st, SeqWP(ss, post))
+    ensures SeqSem([s] + ss, st, post)
+  {
+    forall post': iset<State> | SeqWP(ss, post) <= post' {
+      SemCons(s, st, SeqWP(ss, post), post');
+    }
+  }
+
+  lemma SeqSemNest(ss1: seq<Stmt>, ss2: seq<Stmt>, st: State, post: iset<State>) 
+    requires SeqSem(ss1 + ss2, st, post)
+    ensures SeqSem(ss1, st, SeqWP(ss2, post))
+  {
+    if ss1 == [] {
+      assert [] + ss2 == ss2;
+    } else {
+      assert ([ss1[0]] + (ss1[1..] + ss2))[0] == ss1[0];
+      assert ss1 + ss2 == [ss1[0]] + (ss1[1..] + ss2); 
+    }
+  }
+
+  lemma SeqSemUnNest(ss1: seq<Stmt>, ss2: seq<Stmt>, st: State, post: iset<State>) 
+    requires SeqSem(ss1, st, SeqWP(ss2, post))
+    ensures SeqSem(ss1 + ss2, st, post)
+  {
+    if ss1 == [] {
+      assert [] + ss2 == ss2;
+    } else {
+      assert ([ss1[0]] + (ss1[1..] + ss2))[0] == ss1[0];
+      assert ss1 + ss2 == [ss1[0]] + (ss1[1..] + ss2); 
+    }
+  }
+
+  lemma SeqLemma(ss: seq<Stmt>, cont: seq<Stmt>, st: State, post: iset<State>)
+    requires Sem(Seq(ss + cont), st, post)
+    ensures SeqSem([Seq(ss)] + cont, st, post)
+  {
+    SeqSemNest(ss, cont, st, post);
+    SemUnNest(Seq(ss), cont, st, post);
+  }
+
+  lemma SeqChoiceLemma(s0: Stmt, s1: Stmt, cont: seq<Stmt>, st: State, post: iset<State>)
+    requires SeqSem([s0] + cont, st, post) 
+    requires SeqSem([s1] + cont, st, post)
+    ensures SeqSem([Choice(s0, s1)] + cont, st, post)
+  {
+    SemNest(s0, cont, st, post);
+    SemNest(s1, cont, st, post);
+    SemUnNest(Choice(s0, s1), cont, st, post);
+  }
+
 }
